write down inductive invariant

systems/ChordProof.v
@@ -1,6 +1,7 @@
 Require Import DynamicNet.
 Require Import Chord.
 Require Import List.
+Require Import Arith.
 
 Section ChordProof.
   Variable SUCC_LIST_LEN : nat.
@@ -15,6 +16,10 @@ Section ChordProof.
   Notation timeout_handler := (timeout_handler hash).
 
   Notation global_state := (global_state addr payload data timeout).
+  Notation nodes := (nodes addr payload data timeout).
+  Notation failed_nodes := (failed_nodes addr payload data timeout).
+  Notation sigma := (sigma addr payload data timeout).
+
   Notation step_dynamic := (step_dynamic addr addr_eq_dec payload data timeout timeout_eq_dec start_handler recv_handler timeout_handler client_payload can_be_client can_be_node).
 
   Notation e_timeout := (e_timeout addr payload timeout).
@@ -26,5 +31,100 @@ Section ChordProof.
       t = (e_timeout h (Request dead req)) ->
       (* then it corresponds to an earlier node failure. *)
       In (e_fail dead) xs.
+
+  Definition live_node (gst : global_state) (h : addr) : Prop := exists st,
+    sigma gst h = Some st /\
+    joined st = true /\
+    In h (nodes gst) /\
+    ~ In h (failed_nodes gst).
+
+  Definition live_node_dec (gst : global_state) (h : addr) :=
+    match sigma gst h with
+      | Some st => if joined st
+                   then if in_dec addr_eq_dec h (nodes gst)
+                        then if in_dec addr_eq_dec h (failed_nodes gst)
+                             then false
+                             else true
+                        else false
+                   else false
+      | None => false
+    end.
+
+  Definition best_succ (gst : global_state) (h s : addr) : Prop :=
+    forall st o, exists xs ys,
+      sigma gst h = Some st ->
+      map addr_of (succ_list st) = xs ++ s :: ys ->
+      (In o xs -> ~ live_node gst o) /\
+      live_node gst s.
+
+  (* transitive closure of best_succ *)
+  Inductive reachable (gst : global_state) : addr -> addr -> Prop :=
+    | ReachableSucc : forall from to,
+        best_succ gst from to ->
+        reachable gst from to
+    | ReachableTrans : forall from x to,
+        reachable gst from x ->
+        reachable gst x to ->
+        reachable gst from to.
+
+  Definition best_succ_of (gst : global_state) (h : addr) : option addr :=
+    match (sigma gst) h with
+      | Some st => head (filter (live_node_dec gst) (map addr_of (succ_list st)))
+      | None => None
+    end.
+
+  Definition ring_member (gst : global_state) (h : addr) : Prop :=
+    reachable gst h h.
+
+  Definition at_least_one_ring (gst : global_state) : Prop :=
+    exists h, ring_member gst h.
+
+  Definition at_most_one_ring (gst : global_state) : Prop :=
+    forall x y,
+      ring_member gst x ->
+      ring_member gst y ->
+      reachable gst x y.
+
+  Definition between (x y z : id) :=
+    x < y < z \/ y < z < x \/ z < x < y.
+
+  Lemma between_is_between_bool : forall x y z,
+      between x y z <-> between_bool x y z = true.
+  Admitted.
+
+  Definition ordered_by_id (gst : global_state) (l : list addr) :=
+    forall x y z xs ys,
+      l ++ l = xs ++ x :: y :: z :: ys ->
+      between x y z.
+
+  Definition ordered_ring (gst : global_state) : Prop :=
+    forall h s x,
+      ring_member gst h ->
+      best_succ gst h s ->
+      ring_member gst x ->
+      between h s x \/ s = x.
+
+  Definition connected_appendages (gst : global_state) : Prop :=
+    forall a, exists r,
+      live_node gst a ->
+      ~ ring_member gst a ->
+      ring_member gst r /\ reachable gst a r.
+
+  Definition base_not_skipped (gst : global_state) : Prop :=
+    forall h b succs xs s ys st,
+      live_node gst h ->
+      Some st = sigma gst h ->
+      succs = map addr_of (succ_list st) ->
+      xs ++ s :: ys = succs ->
+      In b base ->
+      between h b s ->
+      In b xs.
+
+  Definition inductive_invariant (gst : global_state) : Prop :=
+    at_least_one_ring gst /\
+    at_most_one_ring gst /\
+    ordered_ring gst /\
+    connected_appendages gst /\
+    base_not_skipped gst.
 
 End ChordProof.
